src/parser/FStarC.Parser.Dep.fsti
@@ -74,7 +74,7 @@ val collect: list string -> (string -> option parsing_data) -> list string & dep
 val deps_of : deps -> string -> list string
 val deps_of_modul : deps -> module_name -> list module_name  // list of modules that this module depends on
 val parsing_data_of: deps -> string -> parsing_data
-val parsing_data_of_modul: deps -> filename:string -> AST.modul -> parsing_data & list string
+val parsing_data_of_modul: deps -> filename:string -> option AST.modul -> parsing_data & list string
 val populate_parsing_data: filename:string -> FStarC.Parser.AST.modul -> dep_graph:deps -> unit
 val print : deps -> unit
 val print_digest: list (string & string) -> string
